messageInvariantPrototypes/twoPhaseCommit/centralized/system.dfy
@@ -4,94 +4,102 @@ include "hosts.dfy"
 module System {
   import opened UtilitiesLibrary
   import opened Types
-  import Host
   import CoordinatorHost
   import ParticipantHost
 
-  datatype Constants = Constants(hosts: seq<Host.Constants>)
+  datatype Constants = Constants(
+    coordinator: seq<CoordinatorHost.Constants>,
+    participants: seq<ParticipantHost.Constants>)
   {
     ghost predicate WF() {
-      Host.GroupWFConstants(hosts)
-    }
-    ghost predicate ValidHostId(id: HostId) {
-      id < |hosts|
+      && CoordinatorHost.GroupWFConstants(coordinator, |participants|)
+      && ParticipantHost.GroupWFConstants(participants)
     }
 
     ghost predicate ValidParticipantId(id: HostId) {
-      id < |hosts|-1
+      id < |participants|
     }
 
-    ghost predicate ValidCoordinatorId(id: HostId) {
-      id == |hosts|-1
+    ghost function GetCoordinator() : CoordinatorHost.Constants 
+      requires WF()
+    {
+      coordinator[0]
     }
   }
 
-  datatype Variables = Variables(hosts: seq<Host.Variables>)
+  datatype Variables = Variables(
+    coordinator: seq<CoordinatorHost.Variables>,
+    participants: seq<ParticipantHost.Variables>
+  )
   {
     ghost predicate WF(c: Constants) {
       && c.WF()
-      && Host.GroupWF(c.hosts, hosts)
+      && CoordinatorHost.GroupWF(c.coordinator, coordinator, |c.participants|)
+      && ParticipantHost.GroupWF(c.participants, participants)
+    }
+
+    ghost function GetCoordinator(c: Constants) : CoordinatorHost.Variables 
+      requires WF(c)
+    {
+      coordinator[0]
     }
   }
 
   ghost predicate Init(c: Constants, v: Variables)
   {
     && v.WF(c)
-    && Host.GroupInit(c.hosts, v.hosts)
+    && CoordinatorHost.GroupInit(c.coordinator, v.coordinator)
+    && ParticipantHost.GroupInit(c.participants, v.participants)
   }
 
   datatype Step =
     | VoteReqStep(coordinator: HostId)
-    | SendVoteStep(participant: HostId, coordinator: HostId, vote: Vote)
-    | DecideStep(coordinator: HostId, decision: Decision)
+    | SendVoteStep(participant: HostId, vote: Vote)
+    | DecideStep(decision: Decision)
     | StutterStep()
 
     
-  ghost predicate NextVoteReqStep(c: Constants, v: Variables, v': Variables, cidx: HostId) 
+  ghost predicate NextVoteReqStep(c: Constants, v: Variables, v': Variables, pidx: HostId) 
     requires v.WF(c) && v'.WF(c)
   {
     var cLbl := CoordinatorHost.VoteReqLbl();
     var pLbl := ParticipantHost.VoteReqLbl();
-    && c.ValidCoordinatorId(cidx)
-    && Host.Next(c.hosts[cidx], v.hosts[cidx], v'.hosts[cidx], Host.CL(cLbl))
-    && (forall pidx:nat | c.ValidParticipantId(pidx)
-        :: Host.Next(c.hosts[pidx], v.hosts[pidx], v'.hosts[pidx], Host.PL(pLbl))
-    )
+    && c.ValidParticipantId(pidx)
+    && ParticipantHost.Next(c.participants[pidx], v.participants[pidx], v'.participants[pidx], pLbl)
+    && CoordinatorHost.Next(c.GetCoordinator(), v.GetCoordinator(c), v'.GetCoordinator(c), cLbl)
+    && (forall x:nat | c.ValidParticipantId(x)
+        ::  v.participants[pidx] == v'.participants[pidx])
   }
 
-  ghost predicate NextSendVoteStep(c: Constants, v: Variables, v': Variables, pidx: HostId, cidx: HostId, vote: Vote) 
+  ghost predicate NextSendVoteStep(c: Constants, v: Variables, v': Variables, pidx: HostId, vote: Vote) 
     requires v.WF(c) && v'.WF(c)
   {
     var cLbl := CoordinatorHost.ReceiveVoteLbl(vote, pidx);
     var pLbl := ParticipantHost.SendVoteLbl(vote);
-    && c.ValidCoordinatorId(cidx)
     && c.ValidParticipantId(pidx)
-    && Host.Next(c.hosts[cidx], v.hosts[cidx], v'.hosts[cidx], Host.CL(cLbl))
-    && Host.Next(c.hosts[pidx], v.hosts[pidx], v'.hosts[pidx], Host.PL(pLbl))
-    && (forall id:nat | c.ValidHostId(id) && id != cidx && id != pidx
-        :: v.hosts[id] == v'.hosts[id]
-    )
+    && CoordinatorHost.Next(c.GetCoordinator(), v.GetCoordinator(c), v'.GetCoordinator(c), cLbl)
+    && ParticipantHost.Next(c.participants[pidx], v.participants[pidx], v'.participants[pidx], pLbl)
+    && (forall x:HostId | c.ValidParticipantId(x)
+        ::  v.participants[x] == v'.participants[x])
   }
 
-  ghost predicate NextDecideStep(c: Constants, v: Variables, v': Variables, cidx: HostId, decision: Decision)
+  ghost predicate NextDecideStep(c: Constants, v: Variables, v': Variables, decision: Decision)
     requires v.WF(c) && v'.WF(c)
   {
     var cLbl := CoordinatorHost.DecideLbl(decision);
     var pLbl := ParticipantHost.DecideLbl(decision);
-    && c.ValidCoordinatorId(cidx)
-    && Host.Next(c.hosts[cidx], v.hosts[cidx], v'.hosts[cidx], Host.CL(cLbl))
-    && (forall pidx:nat | c.ValidParticipantId(pidx)
-        :: Host.Next(c.hosts[pidx], v.hosts[pidx], v'.hosts[pidx], Host.PL(pLbl))
-    )
+    && CoordinatorHost.Next(c.GetCoordinator(), v.GetCoordinator(c), v'.GetCoordinator(c), cLbl)
+    && (forall x:nat | c.ValidParticipantId(x)
+        :: ParticipantHost.Next(c.participants[x], v.participants[x], v'.participants[x], pLbl))
   }
 
   ghost predicate NextStep(c: Constants, v: Variables, v': Variables, step: Step)
     requires v.WF(c) && v'.WF(c)
   {
     match step
-      case VoteReqStep(cidx) => NextVoteReqStep(c, v, v', cidx)
-      case SendVoteStep(pidx, cidx, vote) => NextSendVoteStep(c, v, v', pidx, cidx, vote)
-      case DecideStep(cidx, decision) => NextDecideStep(c, v, v', cidx, decision)
+      case VoteReqStep(pidx) => NextVoteReqStep(c, v, v', pidx)
+      case SendVoteStep(pidx, vote) => NextSendVoteStep(c, v, v', pidx, vote)
+      case DecideStep(decision) => NextDecideStep(c, v, v', decision)
       case StutterStep => v' == v
   }
 
@@ -100,13 +108,6 @@ module System {
     && v.WF(c)
     && v'.WF(c)
     && exists step :: NextStep(c, v, v', step)
-  }
-
-  function GetDecisionForHost(hv: Host.Variables) : Option<Decision>
-  {
-    match hv
-      case CoordinatorVariables(coordinator) => coordinator.decision
-      case ParticipantVariables(participant) => participant.decision
   }
 }
 
