messageInvariantPrototypes/twoPhaseCommit/centralized/applicationProof.dfy
@@ -21,11 +21,11 @@ ghost predicate ApplicationInv(c: Constants, v: Variables)
 ghost predicate LeaderTallyReflectsPreferences(c: Constants, v: Variables)
   requires v.WF(c)
 {
-  var n := |c.hosts|;
-  && (forall hostId | hostId in GetCoordinator(c, v).yesVotes ::
-        0 <= hostId < n-1 && GetParticipantPreference(c, hostId) == Yes )
-  && (forall hostId | hostId in GetCoordinator(c, v).noVotes ::
-        0 <= hostId < n-1 && GetParticipantPreference(c, hostId) == No )
+  var n := |c.participants|;
+  && (forall hostId | hostId in v.GetCoordinator(c).yesVotes ::
+        0 <= hostId < n && GetParticipantPreference(c, hostId) == Yes )
+  && (forall hostId | hostId in v.GetCoordinator(c).noVotes ::
+        0 <= hostId < n && GetParticipantPreference(c, hostId) == No )
 }
 
 // User-level invariant
@@ -35,10 +35,6 @@ ghost predicate Inv(c: Constants, v: Variables)
   && ApplicationInv(c, v)
   && Safety(c, v)
 }
-
-/***************************************************************************************
-*                                        Proof                                         *
-***************************************************************************************/
 
 lemma InvImpliesSafety(c: Constants, v: Variables)
   requires Inv(c, v)
@@ -56,9 +52,21 @@ lemma InvInductive(c: Constants, v: Variables, v': Variables)
   ensures Inv(c, v')
 {
   LeaderTallyReflectsPreferencesInductive(c, v, v');
+  AC1Proof(c, v, v');
   AC3Proof(c, v, v');
   AC4Proof(c, v, v');
 }
+
+/***************************************************************************************
+*                                        Proof                                         *
+***************************************************************************************/
+
+lemma AC1Proof(c: Constants, v: Variables, v': Variables) 
+  requires Inv(c, v)
+  requires Next(c, v, v')
+  ensures SafetyAC1(c, v')
+{}
+
 
 lemma LeaderTallyReflectsPreferencesInductive(c: Constants, v: Variables, v': Variables) 
   requires Inv(c, v)
@@ -74,9 +82,9 @@ lemma AC3Proof(c: Constants, v: Variables, v': Variables)
   requires Next(c, v, v')
   ensures AC3Contrapos(c, v')
 {
-  var n := |c.hosts|;
-  if ! AllPreferYes(c, v) {
-    var noVoter :| 0 <= noVoter < n-1 && c.hosts[noVoter].participant.preference == No;
+  AC3ContraposLemma(c, v);
+  if ! AllPreferYes(c) && CoordinatorHasDecided(c, v') {
+    var noVoter: HostId :| c.ValidParticipantId(noVoter) && c.participants[noVoter].preference == No;
     var sysStep :| NextStep(c, v, v', sysStep);
     if sysStep.DecideStep? {
       var decision := sysStep.decision;
@@ -85,7 +93,16 @@ lemma AC3Proof(c: Constants, v: Variables, v': Variables)
         assert GetParticipantPreference(c, noVoter) == Yes;  // witness
         assert false;
       }
-    } 
+    }
+  }
+}
+
+lemma AC3ContraposLemma(c: Constants, v: Variables)
+  requires Inv(c, v)
+  ensures AC3Contrapos(c, v)
+{
+  if  (!AllPreferYes(c) && CoordinatorHasDecided(c, v)) {
+    assert v.GetCoordinator(c).decision.value != Commit;  // trigger
   }
 }
 
@@ -94,37 +111,30 @@ lemma AC4Proof(c: Constants, v: Variables, v': Variables)
   requires Next(c, v, v')
   ensures SafetyAC4(c, v')
 {
-  if AllPreferYes(c, v') {
-    var n := |v.hosts|;
-    forall i | 0 <= i < n && HostHasDecided(v'.hosts[i]) 
-    ensures HostDecidedCommit(v'.hosts[i]) {
-      var sysStep :| NextStep(c, v, v', sysStep);
-      if sysStep.DecideStep? {
-        /* Proof by contradiction: suppose coord decide no. Then leader's noVotes is
-        not empty. By LeaderTallyReflectsPreferences, this member preferred No, which 
-        contradicts with AllPreferYes(c, v) */
-        var coord := v.hosts[sysStep.coordinator].coordinator;
-        assert coord == GetCoordinator(c, v);  // trigger
-      }
+  if AllPreferYes(c) && CoordinatorHasDecided(c, v'){
+    var sysStep :| NextStep(c, v, v', sysStep);
+    if sysStep.DecideStep? {
+      /* Proof by contradiction: suppose coord decide no. Then leader's noVotes is
+      not empty. By LeaderTallyReflectsPreferences, this member preferred No, which 
+      contradicts with AllPreferYes(c, v) */
     }
   }
 }
 
 lemma YesVotesContainsAllParticipantsWhenFull(c: Constants, v: Variables)
   requires Inv(c, v)
-  requires |Last(v.hosts).coordinator.yesVotes| == |c.hosts|-1
-  ensures forall id | 0 <= id < |c.hosts|-1 :: id in GetCoordinator(c, v).yesVotes
+  requires |v.GetCoordinator(c).yesVotes| == |c.participants|
+  ensures forall id | 0 <= id < |c.participants| :: id in v.GetCoordinator(c).yesVotes
 {
-  var l := GetCoordinator(c, v);
-  forall id | 0 <= id < |c.hosts|-1 
+  var l := v.GetCoordinator(c);
+  forall id | 0 <= id < |c.participants|
   ensures id in l.yesVotes {
     if id !in l.yesVotes {
-      SetLemma(l.yesVotes, id, |c.hosts|-1);
+      SetLemma(l.yesVotes, id, |c.participants|);
       assert false;
     }
   }
 }
-
 
 lemma SetLemma(S: set<HostId>, e: HostId, size: int) 
   requires 0 <= e < size
